DH example compute_message3_proof and decode_message3_proof

examples/dh/DY.Example.DH.Protocol.Total.Proof.fst
@@ -13,7 +13,6 @@ open DY.Example.DH.Protocol.Stateful
 val dh_crypto_usages: crypto_usages
 instance dh_crypto_usages = default_crypto_usages
 
-#push-options "--ifuel 2 --fuel 0"
 val dh_crypto_preds: crypto_predicates dh_crypto_usages
 let dh_crypto_preds = {
   default_crypto_predicates dh_crypto_usages with
@@ -26,14 +25,13 @@ let dh_crypto_preds = {
         exists y. sig_msg2.gy == (dh_pk y) /\ event_triggered tr prin (Respond1 sig_msg2.a prin sig_msg2.gx sig_msg2.gy y)
       )
       | Some (SigMsg3 sig_msg3) -> (
-        exists x. sig_msg3.gx == (dh_pk x) /\ event_triggered tr prin (Initiate2 prin sig_msg3.b sig_msg3.gx sig_msg3.gy x)
+        exists x k. sig_msg3.gx == (dh_pk x) /\ event_triggered tr prin (Initiate2 prin sig_msg3.b sig_msg3.gx sig_msg3.gy k)
       )
       | None -> False
     ))
   );
   sign_pred_later = (fun tr1 tr2 vk msg -> ())
 }
-#pop-options
 
 instance dh_crypto_invs: crypto_invariants = {
   usages = dh_crypto_usages;
@@ -51,7 +49,10 @@ val compute_message1_proof:
       is_secret (principal_state_label alice si) tr x /\
       DhKey? (get_usage x)
     )
-    (ensures is_publishable tr (compute_message1 alice x))
+    (ensures 
+      is_publishable tr (compute_message1 alice x) /\
+      (exists gx. gx == dh_pk x /\ is_publishable tr gx)
+    )
 let compute_message1_proof tr alice bob x si =
   let gx = dh_pk x in
   assert(is_publishable tr gx);
@@ -77,8 +78,7 @@ val decode_message1_proof:
   alice:principal -> bob:principal ->
   msg_bytes:bytes ->
   Lemma
-  (requires bytes_invariant tr msg_bytes /\
-    is_publishable tr msg_bytes)
+  (requires is_publishable tr msg_bytes)
   (ensures (
     match decode_message1 msg_bytes with
     | Some msg1 -> (
@@ -95,8 +95,7 @@ let decode_message1_proof tr alice bob msg_bytes =
       // third argument is applied to the predicate.
       // It then makes sure that the predicate is also true after
       // parsing the third argument from bytes into a data type (message).
-      FStar.Classical.move_requires (parse_wf_lemma message (is_publishable tr)) msg_bytes;
-      FStar.Classical.move_requires (parse_wf_lemma message (bytes_invariant tr)) msg_bytes;
+      parse_wf_lemma message (is_publishable tr) msg_bytes;
       
       // Only for debugging purposes
       assert(bytes_invariant tr msg1.gx);
@@ -105,7 +104,6 @@ let decode_message1_proof tr alice bob msg_bytes =
     )
     | None -> ()
 
-//#push-options "--ifuel 8 --fuel 8 --z3rlimit 25"
 val compute_message2_proof:
   tr:trace -> si:nat ->
   alice:principal -> bob:principal ->
@@ -162,11 +160,10 @@ let compute_message2_proof tr si alice bob msg1 gy y sk_b n_sig =
   let msg = Msg2 {bob; gy; sg} in
   serialize_wf_lemma message (is_publishable tr) msg;
 
-  let msg_bytes = compute_message2 alice bob msg1.gx gy sk_b n_sig in
+  //let msg_bytes = compute_message2 alice bob msg1.gx gy sk_b n_sig in
   //assert(bytes_invariant tr msg_bytes);
   ()
 
-//#push-options "--ifuel 20 --fuel 20 --z3rlimit 100"
 val decode_message2_proof:
   tr:trace ->
   alice:principal -> bob:principal ->
@@ -174,6 +171,7 @@ val decode_message2_proof:
   Lemma
   (requires
     is_publishable tr msg_bytes /\
+    is_publishable tr gx /\
     is_verification_key "DH.SigningKey" (principal_label bob) tr pk_b
   )
   (ensures (
@@ -191,16 +189,18 @@ val decode_message2_proof:
 let decode_message2_proof tr alice bob msg_bytes gx pk_b =
   match decode_message2 msg_bytes alice gx pk_b with
     | Some msg2 -> (
-      FStar.Classical.move_requires (parse_wf_lemma message (is_publishable tr)) msg_bytes;
+      parse_wf_lemma message (is_publishable tr) msg_bytes;
       //FStar.Classical.move_requires (parse_wf_lemma message (bytes_invariant tr)) msg_bytes;
+
+      serialize_wf_lemma sig_message (bytes_invariant tr) (SigMsg2 {a=alice; gx; gy = msg2.gy});
       
-      reveal_opaque (`%verify) (verify);
+      //reveal_opaque (`%verify) (verify);
 
       // Revealing a recursive function does not work with
       // ``reveal_opaque``. That's why we need to use
       // ``normalize_term_spec bytes_invariant;`` or 
       // ``norm_spec [zeta; delta_only [`%bytes_invariant]](bytes_invariant);``
-      normalize_term_spec bytes_invariant;
+      //normalize_term_spec bytes_invariant;
 
       (*assert(bytes_invariant tr msg_bytes);      
       assert(bytes_invariant tr msg2.sg);
@@ -234,6 +234,73 @@ let decode_message2_proof tr alice bob msg_bytes gx pk_b =
         is_corrupt tr (principal_label bob) \/
         (exists y. msg2.gy == dh_pk y /\ event_triggered tr bob (Respond1 alice bob gx msg2.gy y))
       );*)
+      ()
+    )
+    | None -> ()
+
+val compute_message3_proof:
+  tr:trace -> si:nat ->
+  alice:principal -> bob:principal ->
+  msg2:message2 -> gx:bytes -> x:bytes ->
+  sk_a:bytes -> n_sig:bytes ->
+  Lemma
+  (requires
+    (exists k. event_triggered tr alice (Initiate2 alice bob gx msg2.gy k)) /\
+    is_publishable tr gx /\ is_publishable tr msg2.gy /\
+    gx == dh_pk x /\
+    is_signature_key "DH.SigningKey" (principal_label alice) tr sk_a /\
+    is_secret (principal_label alice) tr n_sig /\
+    SigNonce? (get_usage n_sig)
+  )
+  (ensures
+    is_publishable tr (compute_message3 alice bob gx msg2.gy sk_a n_sig)
+  )
+let compute_message3_proof tr si alice bob msg2 gx x sk_a n_sig =
+  let sig_msg = SigMsg3 {b=bob; gx; gy=msg2.gy} in
+  serialize_wf_lemma sig_message (is_publishable tr) sig_msg;
+
+  (* Debugging code
+  assert(is_publishable tr (serialize sig_message sig_msg));*)
+  let sg = sign sk_a n_sig (serialize sig_message sig_msg) in
+
+  (* Debugging code
+  assert(get_label sg `can_flow tr` public);
+  assert(bytes_invariant tr sg);
+  assert(is_publishable tr sg);*)
+
+  let msg = Msg3 {sg} in
+  serialize_wf_lemma message (is_publishable tr) msg;
+
+  (* Debugging code
+  assert(is_publishable tr (serialize message msg));*)
+  ()
+
+val decode_message3_proof:
+  tr:trace -> alice:principal -> bob:principal ->
+  gx:bytes -> gy:bytes -> msg_bytes:bytes -> pk_a:bytes ->
+  Lemma
+  (requires
+    is_publishable tr msg_bytes /\
+    is_publishable tr gx /\
+    is_publishable tr gy /\
+    is_verification_key "DH.SigningKey" (principal_label alice) tr pk_a
+  )
+  (ensures (
+    match decode_message3 msg_bytes bob gx gy pk_a with
+    | Some msg3 -> (
+      let sig_msg = SigMsg3 {b=bob; gx; gy} in
+      is_publishable tr msg3.sg /\
+      verify pk_a (serialize sig_message sig_msg) msg3.sg /\
+      (is_corrupt tr (principal_label alice) \/ is_corrupt tr (principal_label bob) \/
+      (exists x k. gx == dh_pk x /\ event_triggered tr alice (Initiate2 alice bob gx gy k)))
+    )
+    | None -> True
+  ))
+let decode_message3_proof tr alice bob gx gy msg_bytes pk_a =
+  match decode_message3 msg_bytes bob gx gy pk_a with
+    | Some msg3 -> (
+      parse_wf_lemma message (is_publishable tr) msg_bytes;
+      serialize_wf_lemma sig_message (is_publishable tr) (SigMsg3 {b=bob; gx; gy});
       ()
     )
     | None -> ()
